---
aliases: 
creation date: 2023-04-27 14:14
modification date: 2023-04-27 14:14
---

>[!legge]
>Dati $\mathbf{v},\mathbf{w},\mathbf{u}$ vettori liberi allora da $\mathbf{v} + \mathbf{w} = \mathbf{u} + \mathbf{w}$ segue $\mathbf{u} =\mathbf{v}$
>
>>[!dim]
>>Sommando ad ambo i membri $- \mathbf{w}$ otteniamo $$\begin{align}
>>&(\mathbf{v} + \mathbf{w}) + (- \mathbf{w}) = (\mathbf{u} + \mathbf{w}) + (-\mathbf{w}) \implies \mathbf{v} +(\mathbf{w} + (-\mathbf{w})) = \mathbf{u} + (\mathbf{w} + (-\mathbf{w})) \\
>> &\implies \mathbf{v} + \mathbf{0} = \mathbf{u} + \mathbf{0} \implies \mathbf{v} = \mathbf{u}
>>\end{align}$$
>>$\CVD$ 

Da cui possiamo definire la [[differenza]] tra vettori. 